lib/Crypto.lean
@@ -1,6 +1,6 @@
+import Crypto.BitVec
 import Crypto.ByteBuffer
-import Crypto.ByteVec
-import Crypto.Core
+import Crypto.ByteVec2
 import Crypto.UInt8
 import Crypto.Vec
 
@@ -10,27 +10,27 @@ def ByteVec.toBuffer {n:Nat} : ByteVec n → ByteBuffer
 instance : Coe (ByteVec n) ByteBuffer where
   coe := ByteVec.toBuffer
 
---def UInt8.toUInt16 : UInt8 → UInt16 := UInt16.ofNat ∘ UInt8.toNat
---def UInt16.toUInt8 : UInt16 → UInt8 := UInt8.ofNat ∘ UInt16.toNat
-
-def Bit := Bool
-
-def Byte := Vec 8 Bit
-
--- Concatenates a vector together
---def Vec.flatten {α} {m n} : Vec m (Vec n α) → Vec (m * n) α := sorry
-
 structure DRBG where
-  key : ByteVec 32
-  v : ByteVec 16
+  key : BitVec 256
+  v : BitVec 128
 
 instance : Inhabited DRBG := ⟨Inhabited.default, Inhabited.default⟩
 
-@[extern "lean_randombytes_init"]
-constant randombytesInit : @&(ByteVec 48) → DRBG
+open Kind
 
-@[extern "lean_randombytes"]
+@[reducible]
+def Seed := vec 48 (vec 8 bit)
+
+@[extern "lean_random_init"]
+constant randombytesInit : @&Seed → DRBG
+
+@[extern "lean_random_bytes"]
 constant randombytes (rbg:DRBG) (n:@&Nat) : ByteVec n × DRBG
+
+@[extern "lean_random_bits"]
+constant randombits (rbg:DRBG) (n:@&Nat) : BitVec n × DRBG
+
+def mkRandom (drbg:DRBG) (K:Kind) : K × DRBG := randombits drbg K.width
 
 def initKeypairSeedPrefix : ByteVec 1 := #v[64]
 
@@ -66,6 +66,7 @@ def synd_bytes : Nat := ((pk_nrows + 7)/8)
 def PublicKey := ByteVec Mceliece348864Ref.publicKeyBytes
   deriving ToString
 
+@[reducible]
 def SecretKey := ByteVec Mceliece348864Ref.secretKeyBytes
   deriving ToString
 
@@ -80,19 +81,62 @@ structure KeyPair where
   pk : PublicKey
   sk : SecretKey
 
-@[extern "lean_try_crypto_kem_keypair"]
-constant tryCryptoKemKeypair (seed: ByteVec 33) : Option KeyPair × ByteVec 33
+@[extern "lean_shake256"]
+constant shake (w:Nat) (input: ByteArray) : ByteVec w
 
-def mkCryptoKemKeypair (iseed : ByteVec 48) (attempts: optParam Nat 10) : Option (KeyPair × DRBG) := do
-  let rec loop : ∀(seed: ByteVec 33) (attempts:Nat), Option KeyPair
+@[reducible]
+def rw : Nat :=  N/8 + 4*(1 <<< gfbits) + sys_t * 2 + 32
+
+@[extern "lean_load_gf_array"]
+constant loadGfArray (r: ByteVec (2*sys_t)) : ByteVec (2*sys_t) -- FIXME: Make Uint16vec with sys_t elements
+
+@[extern "lean_genpoly_gen"]
+constant genPolyGen (f : ByteVec (2*sys_t)) : Option (ByteVec (2*sys_t))
+
+@[extern "lean_load4_array"]
+constant load4Array (r: ByteVec (4*(1 <<< gfbits))) : ByteVec (4*(1 <<< gfbits)) -- FIXME: Make Uint32vec with (1 <<< gfbits) elements
+
+def irr_bytes : Nat := sys_t * 2
+
+def cond_bytes : Nat := (1 <<< (gfbits-4))*(2*gfbits - 1)
+
+@[extern "lean_store_gf"]
+constant store_gf (irr : ByteVec (2*sys_t)) : ByteVec (2*sys_t)
+
+@[extern "lean_pk_gen"]
+constant pk_gen (sk : ByteVec (2*sys_t)) (perm : ByteVec (4*(1 <<< gfbits)))
+  : Option (PublicKey × ByteVec (2*(1 <<< gfbits)))
+
+@[extern "lean_controlbitsfrompermutation"]
+constant controlBitsFromPermutation (pi : ByteVec (2*(1 <<< gfbits))) : ByteVec cond_bytes
+
+def tryCryptoKemKeypair (seed: ByteVec 32) (r: ByteVec rw) : Option KeyPair := do
+  let sk_input   := r.extractN 0 (N/8)
+  let perm_input := r.extractN (N/8) (4*(1 <<< gfbits))
+  let irr_input  := r.extractN (N/8 + 4*(1 <<< gfbits)) (2*sys_t)
+  let f := loadGfArray irr_input
+  let perm := load4Array perm_input
+  match genPolyGen f with
+  | none => none
+  | some irr =>
+    let sk := store_gf irr
+    match pk_gen sk perm with
+    | none => none
+    | some (pk, pi) =>
+      some ⟨pk, seed ++ ByteVec.ofUInt64lsb 0xffffffff ++ sk ++ controlBitsFromPermutation pi ++ sk_input⟩
+
+def mkCryptoKemKeypair (iseed : Seed) (attempts: optParam Nat 10) : Option (KeyPair × DRBG) := do
+  let rec loop : ∀(seed: ByteVec 32) (attempts:Nat), Option KeyPair
       | _, 0 => none
       | seed, Nat.succ n => do
-        match tryCryptoKemKeypair seed with
-        | ⟨some kp, _⟩ => some kp
-        | ⟨none, seed'⟩ => loop seed' n
+        let r := shake rw (#v[64] ++ seed).data
+        match tryCryptoKemKeypair seed r with
+        | some kp => some kp
+        | none =>
+          loop (r.takeFromEnd 32) n
   let drbg := randombytesInit iseed
   let (bytes, drbg) := randombytes drbg 32
-  match loop (#v[64] ++ bytes) attempts with
+  match loop bytes attempts with
   | none => none
   | some p => some (p, drbg)
 
@@ -100,45 +144,28 @@ structure EncryptionResult where
   ss : Plaintext
   ct : Ciphertext
 
-
 def gfmask : UInt16 := UInt16.ofNat $ (1 <<< gfbits) - 1
 
 def load_gf (src : ByteVec 2) : UInt16 :=
   ((src.get ⟨0, Nat.le.step Nat.le.refl⟩).toUInt16 <<< 8 ||| (src.get ⟨1, Nat.le.refl⟩).toUInt16) &&& gfmask
 
-open Crypto
-
-@[reducible]
-def Byte := vec 8 bit
-
-/-
-def conv1 : Vec (4 * sys_t) Byte → Vec (2 * sys_t) (ByteVec 2) := sorry
-
-def elt1 {n} {α} : Vec n α → i → α := sorry
-
-def gen_e {m} [MonadRandom m] (attempts: optParam Nat 20) : m (ByteVec (N/8)) := do
-  let rec loop : ∀(attempts:Nat), m (ByteVec sys_t)
-      | 0 =>
-        giveUp "Failed to generate error vector."
-      | Nat.succ attempts => do
-        let bytes ← mkRandom (vec (4*sys_t) Byte)
-        let bytes2 := conv1 bytes
-        let nums := load_gf <$> bytes2
-        let nums : Array UInt16 :=
-          Array.generate (2*sys_t) $ λi => load_gf (elt1 bytes2 i) -- .extract (2*i) (2*i+2))
-        pure sorry
-  let v ← loop attempts
-  pure sorry
--/
-
 @[extern "lean_crypto_gen_e_step1"]
-constant gen_e_step1 : @&(ByteVec (4 * sys_t)) → Option (ByteVec (2 * sys_t))
+constant gen_e_step1 : @&(ByteVec (4 * sys_t)) → Option (vec sys_t (vec 16 bit))
 
 @[extern "lean_crypto_gen_e_step2"]
-constant gen_e_step2 : @&(ByteVec (2 * sys_t)) → ByteVec sys_t
+constant gen_e_step2 : @&(vec sys_t (vec 16 bit)) → ByteVec sys_t
 
 @[extern "lean_crypto_gen_e_step3"]
-constant gen_e_step3 : @&(ByteVec (2 * sys_t)) → @&(ByteVec sys_t) → ByteVec (N / 8)
+constant gen_e_step3 : @&(vec sys_t (vec 16 bit)) → @&(ByteVec sys_t) → ByteVec (N / 8)
+
+
+def hasDuplicate (v:vec sys_t (vec 16 bit)) : Bool := Id.run do
+  for i in [0:sys_t] do
+    for j in [0:i] do
+      if v.get! i = v.get! j then
+        return true
+  return false
+
 
 def cGenE2 : ∀(drbg:DRBG) (attempts:Nat), Option (ByteVec (N / 8) × DRBG)
   | _, 0 =>
@@ -168,13 +195,10 @@ def mkCryptoKemEnc (drbg:DRBG) (attempts:Nat) (pk:PublicKey) : Option (Encryptio
 @[extern "lean_decrypt"]
 constant decrypt (ct : @&(ByteVec synd_bytes)) (sk : @&(ByteVec (secretKeyBytes - 40))) : ByteVec (N / 8) × UInt8
 
-def irr_bytes : Nat := sys_t * 2
-
-def cond_bytes : Nat := (1 <<< (gfbits-4))*(2*gfbits - 1)
 
 def cryptoKemDec (c : @&Ciphertext) (sk : @&SecretKey) : Plaintext := Id.run $ do
-  let c_cipher := c.extract 0 synd_bytes
-  let c_hash : ByteVec 32 := c.extract synd_bytes (synd_bytes+32)
+  let c_cipher := c.extractN 0 synd_bytes
+  let c_hash   := c.extractN synd_bytes 32
   let (e, ret_decrypt) := decrypt c_cipher (sk.drop 40)
   let conf := cryptoHash32b (#b[2] ++ e)
   let ret_confirm := ByteVec.orAll (conf ^^^ c_hash)
@@ -183,9 +207,9 @@ def cryptoKemDec (c : @&Ciphertext) (sk : @&SecretKey) : Plaintext := Id.run $ d
   let m := (m >>> 8 : UInt16).toUInt8
 
   -- Generate preimage
-  let s := sk.extract (40 + irr_bytes + cond_bytes) (40 + irr_bytes + cond_bytes + N/8)
+  let s := sk.extractN (40 + irr_bytes + cond_bytes) (N/8)
   let preimageX : ByteVec (N/8) := ~~~m &&& s
-  let preimageY : ByteVec (N/8) := m &&& (e.extract 0 (N/8))
+  let preimageY : ByteVec (N/8) := m &&& (e.extractN 0 (N/8))
   let preimage := preimageX ||| preimageY
   pure $ cryptoHash32b $ #b[m &&& 1] ++ preimage ++ c
 
