lib/Crypto/ByteArray.lean
@@ -22,11 +22,9 @@ def decideEq : (a b : ByteArray) → Decidable (Eq a b) :=
 
 instance : DecidableEq ByteArray := decideEq
 
-@[simp]
 theorem size_push : ∀(a:ByteArray) (b:UInt8), (a.push b).size = a.size + 1
 | ⟨a⟩, b => by simp [ByteArray.size, ByteArray.push]
 
-@[simp]
 theorem size_append : ∀(x y:ByteArray), (x ++ y).size = x.size + y.size
 | ⟨a⟩, ⟨b⟩ => by
   simp [HAppend.hAppend, Append.append, ByteArray.append]
@@ -46,27 +44,144 @@ instance : IsList ByteArray where
   element := UInt8
   fromList := ByteArray.fromList
 
+/-
 @[simp]
 theorem size_empty : size empty = 0 := rfl
 
 @[simp]
 theorem data_empty : empty.data = #[] := rfl
+-/
 
-@[simp]
 theorem size_mkEmpty (n:Nat) : size (mkEmpty n) = 0 := rfl
 
 theorem size_fromListAux : ∀(l:List UInt8) (r:ByteArray), (fromListAux l r).size = r.size + l.length
 | [] , r => rfl
-| a :: as, r => by simp [fromListAux, size_fromListAux as _, Nat.add_succ, Nat.succ_add] 
+| a :: as, r => by simp [fromListAux, size_fromListAux as _, Nat.add_succ, Nat.succ_add, size_push]
 
-@[simp]
 theorem size_from_list : ∀(l:List UInt8), ByteArray.size (fromList l) = l.length
 | [] => rfl
-| a :: as => by simp [fromList, IsList.fromList, ByteArray.fromList, size_fromListAux] 
+| a :: as => by simp [fromList, IsList.fromList, ByteArray.fromList, size_fromListAux, size_mkEmpty]
+
+def replicateAux : ByteArray → Nat → UInt8 → ByteArray
+| a, 0, _ => a
+| a, Nat.succ n, c => replicateAux (a.push c) n c
+
+def replicate (n:Nat) (c:UInt8) : ByteArray := replicateAux (ByteArray.mkEmpty n) n c
+
+theorem size_replicateAux (a:ByteArray) (n:Nat) (c:UInt8) : (replicateAux a n c).size = a.size + n := by
+  revert a
+  induction n with
+  | zero =>
+    intro a
+    simp [replicateAux]
+  | succ n nh =>
+    intro a
+    simp [replicateAux, nh, ByteArray.size_push, Nat.add_succ, Nat.succ_add]
+
+theorem size_replicate (n:Nat) (c:UInt8) : (replicate n c).size = n := by
+  simp [replicate, size_replicateAux, size_mkEmpty]
+
+def sequenceAux : ByteArray → Nat → ByteArray
+| a, 0 => a
+| a, Nat.succ n => sequenceAux (a.push (UInt8.ofNat a.size)) n
+
+-- Creates a vector [0..n)
+def sequence (n:Nat) : ByteArray := sequenceAux (ByteArray.mkEmpty n) n
+
+theorem size_sequenceAux (a:ByteArray) (n:Nat) : (sequenceAux a n).size = a.size + n := by
+  revert a
+  induction n with
+  | zero =>
+    intro a
+    simp [sequenceAux]
+  | succ n nh =>
+    intro a
+    simp [sequenceAux, nh, ByteArray.size_push, Nat.add_succ, Nat.succ_add]
+
+theorem size_sequence (n:Nat) : (sequence n).size = n := by
+  simp [sequence, size_sequenceAux, size_mkEmpty]
 
 theorem size_extract : ∀(a:ByteArray) (s e : Nat), (a.extract s e).size = min e a.size - s
 | ⟨a⟩, s, e => by
-  simp [extract, copySlice]
-  admit
+  simp [extract, copySlice, size, empty, mkEmpty, Array.size_empty, min]
+  cases Decidable.em (e ≤ Array.size a) with
+  | inl h1 =>
+    cases Decidable.em (s ≤ e) with
+    | inl h2 =>
+      simp [h1, Nat.add_sub_of_le h2]
+    | inr h2 =>
+      have s3 := Nat.le_of_lt (Nat.gt_of_not_le h2)
+      simp [h1, Nat.le_implies_zero_sub, s3]
+      cases Decidable.em (s ≤ a.size) with
+      | inl h3 =>
+        simp [h3]
+      | inr h3 =>
+        have s3 := Nat.le_of_lt (Nat.gt_of_not_le h3)
+        simp [Nat.le_implies_zero_sub, s3, h3]
+  | inr h1 =>
+    cases Decidable.em (s ≤ e) with
+    | inl h2 =>
+      simp [h1, Nat.add_sub_of_le h2]
+    | inr h2 =>
+      have n_le_s : e ≤ s := Nat.le_of_lt (Nat.gt_of_not_le h2)
+      simp [h1, Nat.le_implies_zero_sub, n_le_s]
+      cases Decidable.em (s ≤ a.size) with
+      | inl h3 =>
+        have h11 : a.size ≤ e := Nat.le_of_lt (Nat.gt_of_not_le h1)
+        have h31 : a.size ≤ s := Nat.le_trans h11 n_le_s
+        simp [h3, Nat.le_implies_zero_sub, h31]
+      | inr h3 =>
+        simp [h3]
+
+def extractN (a:ByteArray) (s n : Nat) : ByteArray :=
+  let b := a.extract s (s+n)
+  b ++ replicate (n-b.size) 0
+
+theorem size_extractN (a:ByteArray) (s n : Nat) : (a.extractN s n).size = n := by
+  simp [extractN, size_append, size_extract, size_replicate, min]
+  cases Decidable.em (s + n ≤ a.size) with
+  | inl h1 =>
+    simp [h1, Nat.add_sub_self_left]
+  | inr h1 =>
+    have h11 : a.size ≤ s+n := Nat.le_of_lt (Nat.gt_of_not_le h1)
+    have p : a.size - s ≤ n := by
+           apply Nat.le_sub_of_le_add
+           rw [Nat.add_comm]
+           exact h11
+    have q := Nat.add_sub_of_le p
+    simp [h1, q]
+
+
+def generateAux {n:Nat} (f:Fin n → UInt8) : ∀(a:ByteArray) (j : Nat), a.size + j = n → ByteArray
+| a, 0, p => a
+| a, Nat.succ j, p =>
+  let q : a.size < n := by
+    apply Nat.add_le_implies_le_rhs j
+    apply Nat.le_of_eq
+    rw [Nat.add_comm]
+    simp [Nat.succ_add]
+    exact p
+  let r : (a.push (f ⟨a.size, q⟩)).size + j = n := by
+        simp [size_push, Nat.add_succ, Nat.succ_add]
+        exact p
+  generateAux f (a.push (f ⟨a.size, q⟩)) j r
+
+def generate (n:Nat) (f:Fin n → UInt8) : ByteArray :=
+  let p : (mkEmpty n).size + n = n := by simp [size_mkEmpty]
+  generateAux f (mkEmpty n) n p
+
+theorem size_generateAux {n:Nat} (f:Fin n → UInt8) {a:ByteArray} (j:Nat) (p:a.size + j = n)
+    : (generateAux f a j p).size = n := by
+  revert a p
+  induction j with
+  | zero =>
+    intros a p
+    exact p
+  | succ j ind =>
+    intros a p
+    exact ind _
+
+theorem size_generate (n:Nat) (f:Fin n → UInt8) : (generate n f).size = n := by
+  exact (size_generateAux _ _ _)
 
 end ByteArray
