lib/Crypto/IsList.lean
@@ -1,5 +1,5 @@
 class IsList (α : Type) where
   element : Type
-  fromList {} : List element → α 
+  fromList : List element → α
 
 export IsList (fromList)
