lakefile.lean
@@ -28,9 +28,7 @@ def bindingsTarget (pkgDir : FilePath) : FileTarget  :=
       "c++"
 
 def mcelieceFiles : Array FilePath :=
-  let nist : FilePath := "nist"
-  #[ nist / "rng.c",
-     "benes.c", "bm.c", "controlbits.c", "decrypt.c", "encrypt.c", "gf.c",
+  #[ "benes.c", "bm.c", "controlbits.c", "decrypt.c", "encrypt.c", "gf.c",
      "pk_gen.c", "root.c", "sk_gen.c", "synd.c", "transpose.c", "util.c"
     ]
 
