lib/Crypto/Array.lean
@@ -11,35 +11,38 @@ theorem ite_same {α:Type} (p:Prop) [h:Decidable p] (a:α) : (if p then a else a
   | isFalse q => simp [q]
   | isTrue q => simp [q]
 
-theorem size_foldlM_loop {α:Type} (b:Array α) (stop:Nat) (h:stop ≤ b.size) (i j : Nat) (inv : i = stop - j) (a : Array α)
+theorem size_foldlM_loop {α:Type} (b:Array α) (stop:Nat) (h:stop ≤ b.size) (i j : Nat)
+  (inv : i = stop - j) (a : Array α)
 : size (Id.run (foldlM.loop (fun r v => push r v) b stop h i j a)) = a.size + i := by
-  simp [Id.run, foldlM.loop]
   revert j a
   induction i with
-  | zero => 
+  | zero =>
     intros j inv a
-    simp [foldlM.loop]
-    cases Decidable.em (j < stop) with
+    rw [Id.run, foldlM.loop]
+    cases Decidable.em (j< stop) with
     | inl q => simp [q]
     | inr q => simp [q]
-  | succ i ih => 
+  | succ i ih =>
     intros j inv a
-    simp [foldlM.loop]
+    rw [foldlM.loop]
     have q : j < stop := Nat.sub_pos_implies_lt inv
-    have r : i = stop - (j + 1) := by 
+    simp [q]
+    have r : i = stop - (j + 1) := by
       apply Nat.add_implies_sub q
       have q_leq : j ≤ stop := Nat.le_of_lt q
       have s : Nat.succ i + j = stop := Nat.sub_implies_add q_leq inv
       simp [Nat.succ_add] at s
       exact s
-    simp [q, ih (j+1) r, Nat.succ_add, Nat.add_succ]      
+    simp [ih (Nat.succ j) r, Nat.succ_add, Nat.add_succ]
 
 @[simp]
 theorem size_append {α:Type} : ∀(x y:Array α), (x ++ y).size = x.size + y.size
 | a, b => by
   simp [HAppend.hAppend, Append.append, Array.append, Array.foldl]
   have h : size b ≤ size b := Nat.le.refl
-  simp [foldlM, h, size_foldlM_loop]    
+  simp [foldlM, h, size_foldlM_loop]
+
+--  simp [foldlM, h, size_foldlM_loop]
 
 @[simp]
 theorem size_ofSubarray {α:Type} (s:Subarray α) : (ofSubarray s).size = s.stop - s.start := sorry
@@ -53,23 +56,23 @@ theorem start_toSubarray_large {α:Type} (a:Array α) (start stop : Nat) (p : a.
   : (toSubarray a start stop).start = a.size := by
     simp only [toSubarray]
     cases Decidable.em (stop ≤ size a) with
-    | inl g => 
+    | inl g =>
       simp [g]
       cases Decidable.em (start ≤ stop) with
-      | inl h =>       
+      | inl h =>
         simp [h]
         have r : start ≤ size a := Nat.le_trans h g
         exact (Nat.le_antisymm r p)
-      | inr h =>       
+      | inr h =>
         simp [h]
         exact (Nat.le_antisymm g q)
-    | inr g => 
+    | inr g =>
       simp [g]
       cases Decidable.em (start ≤ a.size) with
       | inl h =>
         simp [h]
         exact (Nat.le_antisymm h p)
-      | inr h => 
+      | inr h =>
         simp [h]
 
 @[simp]
@@ -77,16 +80,16 @@ theorem stop_toSubarray_large {α:Type} (a:Array α) (start stop : Nat) (p : a.s
   : (toSubarray a start stop).stop = a.size := by
     simp only [toSubarray]
     cases Decidable.em (stop ≤ size a) with
-    | inl g => 
+    | inl g =>
       simp [g]
       cases Decidable.em (start ≤ stop) with
       | inl h =>
         simp [h]
         exact (Nat.le_antisymm g q)
-      | inr h =>       
+      | inr h =>
         simp [h]
         exact (Nat.le_antisymm g q)
-    | inr g => 
+    | inr g =>
       simp [g]
       cases Decidable.em (start ≤ a.size) with
       | inl h => simp [h]
@@ -96,27 +99,27 @@ theorem stop_toSubarray_large {α:Type} (a:Array α) (start stop : Nat) (p : a.s
 theorem stop_toSubarray {α:Type} (a:Array α) (start stop : Nat) (p : start ≤ stop) (q : stop ≤ a.size)
   : (toSubarray a start stop).stop = stop := by simp [toSubarray, p, q]
 
-theorem size_empty : Array.size (#[] : Array UInt8) = 0 := by rfl
+theorem size_empty {tp:Type} : Array.size (#[] : Array tp) = 0 := by rfl
 
 @[simp]
-theorem size_extract {α:Type} (src: Array α) (start stop : Nat) 
+theorem size_extract {α:Type} (src: Array α) (start stop : Nat)
 : (src.extract start stop).size = min stop src.size - start := by
   simp [extract, toSubarray]
   cases Decidable.em (stop ≤ size src) with
-  | inl g => 
+  | inl g =>
     simp [g, min]
     cases Decidable.em (start ≤ stop) with
     | inl h => simp [h]
-    | inr h => 
+    | inr h =>
       have q := Nat.gt_of_not_le h
-      simp [h, Nat.sub_self, Nat.lt_implies_zero_sub q]      
-  | inr g => 
+      simp [h, Nat.sub_self, Nat.lt_implies_zero_sub q]
+  | inr g =>
     simp [g, min]
     cases Decidable.em (start ≤ size src) with
     | inl h =>
       simp [h]
-    | inr h => 
+    | inr h =>
       have q := Nat.gt_of_not_le h
-      simp [h, Nat.sub_self, Nat.lt_implies_zero_sub q]  
+      simp [h, Nat.sub_self, Nat.lt_implies_zero_sub q]
 
 end Array
