lib/Crypto/BitVec.lean
@@ -1,0 +1,35 @@
+import Crypto.ByteArray
+import Crypto.UInt8
+
+structure BitVec (n:Nat) where
+  data : ByteArray
+  size_proof : data.size = (n+7)/8
+
+namespace BitVec
+
+protected def zeros (n:Nat) : BitVec n := ⟨ByteArray.replicate ((n+7)/8) 0, by simp [ByteArray.size_replicate]⟩
+
+instance (n:Nat) : Inhabited (BitVec n) := ⟨BitVec.zeros n⟩
+
+-- Get with most-significant bit first.
+protected def get! (x:BitVec n) (i:Nat) : Bool :=
+  let off := i / 8
+  let byte := x.data.get! off
+  let mod := UInt8.ofNat (i % 8)
+  let mask := 1 <<< (7 - mod)
+  (byte &&& mask) == mask
+
+
+protected def toHex {n:Nat} (a:BitVec n) : String := a.data.foldl (λs b => s ++ b.toHex) ""
+
+protected def toString {n:Nat} (a:BitVec n) : String :=
+  if n % 4 == 0 then
+    "Ox" ++ a.toHex
+  else
+    let firstByte := a.data.get! 0
+    let startStr := "0b" ++ firstByte.toBits (n % 8)
+    a.data.foldl (λs b => s ++ b.toBits) startStr 1
+
+instance (n:Nat) : ToString (BitVec n) := ⟨BitVec.toString⟩
+
+end BitVec
