lib/Crypto/Core.lean
@@ -1,3 +1,4 @@
+/-
 import Crypto.Vec
 
 namespace Crypto
@@ -32,3 +33,4 @@ export MonadRandom(mkRandom)
 export MonadRandom(giveUp)
 
 end Crypto
+-/
